theories/rules/rules_EInit.v
@@ -55,7 +55,7 @@ Section cap_lang_rules.
     ⌜is_valid_updated_lmemory glmem lmem (finz.seq_between data_b data_e) data_v lmem'' ⌝ ∗ (* all memory in the data capability is "current" w.r.t. revocation *)
     ⌜ lmem' =
     <[ ( data_b, (data_v+1)%nat ) := (LSealRange (true,true) ot (ot ^+ 2)%ot ot ) ]>
-      (<[ (code_b, code_v) := (LCap RW data_b data_e data_a (data_v + 1)%nat) ]> lmem'') ⌝ ∗
+      (<[ (code_b, (code_v+1)%nat ) := (LCap RW data_b data_e data_a (data_v + 1)%nat) ]> lmem'') ⌝ ∗
     ⌜unique_in_registersL lregs (Some r_code) (LCap RX code_b code_e code_a code_v) ⌝ ∗ (* the code capability is unique across all registers (except where it is stored: in `r_code`) *)
     ⌜unique_in_registersL lregs (Some r_data) (LCap RW data_b data_e data_a data_v) ⌝ ∗ (* the data capability is unique across all registers (except where it is stored: in `r_code`) *)
     ⌜ map_Forall (fun la lw => (laddr_get_addr la) ∈ (finz.seq_between (code_b ^+ 1)%a code_e) -> is_zL lw) lmem⌝ ∗
